Change substitutions from lists of pairs to functions from nats to patterns

LeanChecker/Pattern.lean
@@ -1,4 +1,3 @@
-
 inductive Pattern where
     | metavar(id: Nat) : Pattern
     | bot : Pattern --- TODO: Replace with $mu X. X$ Not needed by $phi -> phi$
@@ -12,23 +11,30 @@ def ph1 : Pattern := (Pattern.metavar 1)
 def ph2 : Pattern := (Pattern.metavar 2)
 def ph0_implies_ph0 : Pattern := (implies ph0 ph0)
 
-def Pattern.instantiate(p: Pattern)(subst: List (Nat × Pattern)) : Pattern :=
+def subst_from_pairs(pairs: List (Nat × Pattern))(n: Nat): Option Pattern :=
+    match pairs with
+        | [] => none
+        | (x, p) :: xs => if x = n then p else (subst_from_pairs xs n)
+
+/-- Inhabited `get` function. Returns `a` if the input is `some a`, otherwise returns `default`. -/
+def Option.get_or_default (opt: Option α) (default: α) : α :=
+  match opt with
+  | some x => x
+  | none => default
+
+def Pattern.instantiate(p: Pattern)(subst: Nat -> Option Pattern) : Pattern :=
     match p with
-      | Pattern.metavar id' =>
-            match subst with
-             | [] => p
-             | (id, plug) :: rest
-                => if id' = id then plug else p.instantiate rest
+      | Pattern.metavar id' =>  (subst id').get_or_default p
       | Pattern.bot => Pattern.bot
       | Pattern.implies left right => Pattern.implies (left.instantiate subst) (right.instantiate subst)
 
 theorem test_inst_1 :
-    (Pattern.instantiate Pattern.bot [(0, ph0)]) = Pattern.bot := by rfl
+    (Pattern.instantiate Pattern.bot  $ subst_from_pairs [(0, ph0)]) = Pattern.bot := by rfl
 theorem test_inst_2 :
-    (Pattern.instantiate ph0 [(0, ph0)]) = ph0 := by rfl
+    (Pattern.instantiate ph0 $ subst_from_pairs [(0, ph0)]) = ph0 := by rfl
 theorem test_inst_3 :
-    (Pattern.instantiate ph1 [(0, ph0)]) = ph1 := by rfl
+    (Pattern.instantiate ph1 $ subst_from_pairs [(0, ph0)]) = ph1 := by rfl
 theorem test_inst_4 :
-    (Pattern.instantiate ph0_implies_ph0 [(0, ph1)]) = (implies ph1 ph1) := by rfl
+    (Pattern.instantiate ph0_implies_ph0 $ subst_from_pairs [(0, ph1)]) = (implies ph1 ph1) := by rfl
 theorem test_inst_5 :
-    (Pattern.instantiate ph0_implies_ph0 [(0, ph0_implies_ph0)]) = (implies ph0_implies_ph0 ph0_implies_ph0) := by rfl
+    (Pattern.instantiate ph0_implies_ph0 $ subst_from_pairs [(0, ph0_implies_ph0)]) = (implies ph0_implies_ph0 ph0_implies_ph0) := by rfl
